get started with live loops

bedrock2/src/bedrock2/OperatorOverloading.v
@@ -24,6 +24,7 @@ Require Import bedrock2.Scalars.
 
 Class PointsTo{width: Z}{word: word.word width}{mem: map.map word Byte.byte}{V: Type}
       (addr: word)(val: V)(pred: mem -> Prop) := {}.
+Global Hint Mode PointsTo + + + + + + - : typeclass_instances.
 
 (* Precedence: `*` is at level 40, and we want to bind stronger than `*`, and moreover,
    `^` is at level 30, and for consistency, we also want to bind stronger than `^`,
@@ -33,6 +34,12 @@ Notation "a ~> v" := (infer! PointsTo a v)
 
 Class PointsToPredicate{width}{word: word.word width}{mem: map.map word Byte.byte}
       (V: Type)(pred: word -> V -> mem -> Prop) := {}.
+Global Hint Mode PointsToPredicate + + + + - : typeclass_instances.
+
+(* separate typeclass because some predicates don't have a constant size *)
+Class PredicateSize{width}{word: word.word width}{mem: map.map word Byte.byte}{V: Type}
+      (pred: word -> V -> mem -> Prop){p: PointsToPredicate V pred}(sz: Z) := {}.
+Global Hint Mode PredicateSize + + + + - - - : typeclass_instances.
 
 #[export] Instance PointsToPredicate_to_PointsTo
  {width}{word: word.word width}{mem: map.map word Byte.byte}{V: Type}
@@ -44,10 +51,6 @@ Class PointsToPredicate{width}{word: word.word width}{mem: map.map word Byte.byt
   PointsToPredicate word scalar := {}.
 Notation "a ~> v" := (scalar a v)
   (at level 25, format "'[  ' a  ~>  '/' v ']'", only printing) : oo_scope.
-
-Class PredicateSize{width}{word: word.word width}{mem: map.map word Byte.byte}{V: Type}
-      (pred: word -> V -> mem -> Prop){p: PointsToPredicate V pred}(sz: Z) := {}.
-
 #[export] Instance Scalar32Size{word: word.word 32}{mem: map.map word Byte.byte}:
   PredicateSize (scalar (word := word)) 4 | 5 := {}.
 #[export] Instance Scalar64Size{word: word.word 64}{mem: map.map word Byte.byte}:
@@ -55,6 +58,13 @@ Class PredicateSize{width}{word: word.word width}{mem: map.map word Byte.byte}{V
 #[export] Instance ScalarGenericSize
  {width: Z}{word: word.word width}{mem: map.map word Byte.byte}:
   PredicateSize (scalar (word := word)) (Memory.bytes_per_word width) | 6 := {}.
+
+#[export] Instance PointsToBytePredicate
+ {width}{word: word.word width}{mem: map.map word Byte.byte}:
+  PointsToPredicate Byte.byte (ptsto (map := mem)) := {}.
+Notation "a ~> v" := (ptsto a v) (only printing) : oo_scope.
+#[export] Instance PtstoSize{width: Z}{word: word.word width}{mem: map.map word Byte.byte}:
+  PredicateSize (ptsto (map := mem)) 1 := {}.
 
 
 Require Import bedrock2.Array.
