bedrock2/src/bedrock2Examples/LiveVerif/LiveVerif.v
@@ -35,8 +35,6 @@ Section LiveVerif.
   Local Set Implicit Arguments.
   Local Open Scope string_scope. Local Open Scope Z_scope. Local Open Scope list_scope.
   Local Open Scope sep_bullets_scope.
-  Coercion Z.of_nat : nat >-> Z.
-  Coercion byte.unsigned : byte >-> Z.
   Notation len := List.length.
   Notation "'bytetuple' sz" := (HList.tuple byte (@Memory.bytes_per 32 sz)) (at level 10).
   Local Open Scope oo_scope.
